src/tls/TLSExtensions.fst
@@ -10,7 +10,7 @@ open TLSError
 open TLSConstants
 open TLSInfo
 open CoreCrypto
-
+let op_At = FStar.List.Tot.append
 type renegotiationInfo =
   | FirstConnection
   | ClientRenegotiationInfo of (cVerifyData)
@@ -43,7 +43,7 @@ let parseRenegotiationInfo b =
     | Error(z) -> Error(AD_decode_error, perror __SOURCE_FILE__ __LINE__ "Failed to parse renegotiation info length")
   else Error (AD_decode_error, perror __SOURCE_FILE__ __LINE__ "Renegotiation info bytes are too short")
 
-type preEarlyDataIndication =
+type preEarlyDataIndication : Type0 =
   { ped_configuration_id: configurationId;
     ped_cipher_suite:cipherSuite;
     ped_extensions:list extension;
